whitespace etc

src/DFS.v
@@ -4,394 +4,389 @@ From coqutil Require Import Tactics.destr Tactics.Tactics Tactics.fwd.
 From GraphSearch Require Import List GraphInterface.
 Import ListNotations.
 
-
 Section __.
   Context {V : Type}.
-
-
   Context {eqbV : Eqb V}.
   Context {graph : graph.graph V}.
   Context {ok : graph.ok graph}.
   Context {eqb_ok : Eqb_ok eqbV}.
 
-  Section fold.
-    Context {state : Type}.
-    Context (untree_edge_upd : state -> list V -> V -> state).
-    Context (tree_edge_upd : state -> list V -> V -> state).
-    Context (finish : state -> list V -> V -> state).
+  Context {state : Type}.
+  Context (untree_edge_upd : state -> list V -> V -> state).
+  Context (tree_edge_upd : state -> list V -> V -> state).
+  Context (finish : state -> list V -> V -> state).
+
+  Section with_graph.
+    Context (g : graph).
 
 
-    Section with_graph.
-      Context (g : graph).
+    Definition state' : Type := list V * state.
+    Definition untree_edge_upd' '(vs, st) v := (vs, untree_edge_upd st vs v).
+    Definition tree_edge_upd' '(vs, st) v := (v :: vs, tree_edge_upd st vs v).
+    Definition finish' '(vs, st) v := (vs, finish st vs v).
+
+    Definition already_seen (st' : state') v :=
+      let '(vs, _) := st' in set_contains vs v.
+
+    Fixpoint dfs_fold' n st' v : state' :=
+      match n with
+      | S n' =>
+          if already_seen st' v then untree_edge_upd' st' v else
+            finish' (fold_left (dfs_fold' n') (graph.edges g v) (tree_edge_upd' st' v)) v
+      | O => st'
+      end.
+
+    Definition dfs_fold st0 := dfs_fold' (3 + length (graph.sources g)) ([], st0).
+  End with_graph.
+
+  Inductive dfs_fold_state (root : V) vs0 st0 : list V (*seen*) -> state -> list V (*current path*)-> graph (*explored edges*) -> Prop :=
+  | dfs_init : dfs_fold_state _ _ _ vs0 st0 [root] graph.empty
+  | dfs_tree_edge vs st u p g v :
+    ~graph.edge g u v ->
+    dfs_fold_state _ _ _ vs st (u :: p) g ->
+    set_contains vs v = false ->
+    dfs_fold_state _ _ _ (v :: vs) (tree_edge_upd st vs v) (v :: u :: p) (graph.put g u v)
+  | dfs_untree_edge vs st u p g v :
+    dfs_fold_state _ _ _ vs st (u :: p) g ->
+    ~graph.edge g u v ->
+    set_contains vs v = true ->
+    dfs_fold_state _ _ _ vs (untree_edge_upd st vs v) (u :: p) (graph.put g u v)
+  | dfs_finish vs st u p g :
+    dfs_fold_state _ _ _ vs st (u :: p) g ->
+    dfs_fold_state _ _ _ vs (finish st vs u) p g.
+
+  Lemma set_contains_cons_true v vs y :
+    set_contains vs y = true -> set_contains (v :: vs) y = true.
+  Proof. rewrite !set_contains_true. simpl. auto. Qed.
+
+  Lemma set_contains_head v vs :
+    set_contains (v :: vs) v = true.
+  Proof. apply set_contains_true. left. reflexivity. Qed.
+
+  Lemma seen_mono root vs0 st0 vs st p g y :
+    dfs_fold_state root vs0 st0 vs st p g ->
+    set_contains vs0 y = true ->
+    set_contains vs y = true.
+  Proof. intros H Hy. induction H; auto using set_contains_cons_true. Qed.
+
+  Lemma seen_mono' root vs0 st0 vs st p g :
+    dfs_fold_state root vs0 st0 vs st p g ->
+    incl vs0 vs.
+  Proof.
+    intros H x Hx. apply set_contains_true. eapply seen_mono; try eassumption.
+    apply set_contains_true. exact Hx.
+  Qed.
+
+  Hint Unfold graph.edge : core.
+  Lemma dfs_target_seen root vs0 st0 vs st p g x y :
+    dfs_fold_state root vs0 st0 vs st p g -> graph.edge g x y -> set_contains vs y = true.
+  Proof.
+    intro H. revert x y.
+    induction H; intros x y He.
+    - apply graph.edge_empty in He. contradiction.
+    - apply graph.edge_put in He. destruct He as [Hold | [_ Hvy]].
+      + apply set_contains_cons_true. eauto.
+      + subst y. apply set_contains_head.
+    - apply graph.edge_put in He. destruct He as [Hold | [_ Hvy]].
+      + eauto.
+      + subst y. assumption.
+    - eauto.
+  Qed.
+
+  Lemma dfs_path_seen root vs0 st0 vs st p g z :
+    set_contains vs0 root = true ->
+    dfs_fold_state root vs0 st0 vs st p g ->
+    In z p ->
+    set_contains vs z = true.
+  Proof.
+    intros Hroot H. revert z.
+    induction H; intros z Hz.
+    - destruct Hz as [<- | []]. exact Hroot.
+    - destruct Hz as [<- | Hz].
+      + apply set_contains_head.
+      + apply set_contains_cons_true. eauto.
+    - eauto.
+    - eauto using in_cons.
+  Qed.
+
+  Lemma dfs_path_unseen root vs0 st0 vs st p g z :
+    dfs_fold_state root vs0 st0 vs st p g -> In z p -> z = root \/ set_contains vs0 z = false.
+  Proof.
+    intro H. revert z.
+    induction H; intros z Hz.
+    - destruct Hz as [<- | []]. left. reflexivity.
+    - destruct Hz as [<- | Hz].
+      + right. apply set_contains_false. intro Hin.
+        match goal with He : dfs_fold_state _ _ _ _ _ _ _ |- _ =>
+                          apply (seen_mono' _ _ _ _ _ _ _ He) in Hin end.
+        apply set_contains_true in Hin. congruence.
+      + eauto.
+    - eauto.
+    - eauto using in_cons.
+  Qed.
+
+  Lemma dfs_source_seen root vs0 st0 vs st p g x y :
+    set_contains vs0 root = true ->
+    dfs_fold_state root vs0 st0 vs st p g -> graph.edge g x y -> set_contains vs x = true.
+  Proof.
+    intros Hroot H. revert x y.
+    induction H; intros x y He.
+    - apply graph.edge_empty in He. destruct He.
+    - apply graph.edge_put in He. destruct He as [Hold | [Hxhd _]].
+      + apply set_contains_cons_true. eauto.
+      + subst x. apply set_contains_cons_true.
+        eapply dfs_path_seen; [ exact Hroot | eassumption | apply in_eq ].
+    - apply graph.edge_put in He. destruct He as [Hold | [Hxhd _]].
+      + eauto.
+      + subst x. eapply dfs_path_seen; [ exact Hroot | eassumption | apply in_eq ].
+    - eauto.
+  Qed.
+
+  Lemma dfs_fold_state_trans root vs0 st0 vs st vs' st' p p' g g' u :
+    dfs_fold_state root vs0 st0 vs st (u :: p) g ->
+    set_contains vs0 root = true ->
+    graph.edges g u = [] ->
+    dfs_fold_state u vs st vs' st' p' g' ->
+    dfs_fold_state root vs0 st0 vs' st' (p' ++ p) (graph.union g g').
+  Proof.
+    intros H1 Hroot Hedges H2.
+    induction H2.
+    - cbn [app]. rewrite graph.union_empty_r. exact H1.
+    - cbn [app]. rewrite graph.union_put_r. apply dfs_tree_edge.
+      + intro Hedge. apply graph.edge_union in Hedge. destruct Hedge as [Hg | Hg0].
+        * pose proof (dfs_target_seen _ _ _ _ _ _ _ _ _ H1 Hg) as Hs.
+          match goal with He : dfs_fold_state u _ _ _ _ _ _ |- _ =>
+                            pose proof (seen_mono _ _ _ _ _ _ _ _ He Hs) end.
+          congruence.
+        * contradiction.
+      + eassumption.
+      + eassumption.
+    - cbn [app]. rewrite graph.union_put_r. apply dfs_untree_edge.
+      + eassumption.
+      + intro Hedge. apply graph.edge_union in Hedge. destruct Hedge as [Hg | Hg0].
+        * match goal with He : dfs_fold_state u _ _ _ _ _ _ |- _ =>
+                            pose proof (dfs_path_unseen _ _ _ _ _ _ _ _ He (in_eq _ _)) as Hun end.
+          destruct Hun as [-> | Hun].
+          -- cbv [graph.edge] in Hg. rewrite Hedges in Hg. destruct Hg.
+          -- pose proof (dfs_source_seen _ _ _ _ _ _ _ _ _ Hroot H1 Hg) as Hsn. congruence.
+        * contradiction.
+      + eassumption.
+    - eapply dfs_finish. eassumption.
+  Qed.
+
+  Definition graph_corresp vs vs' (g g_acc : graph) :=
+    (forall s, In s (graph.sources g_acc) -> In s vs'/\  ~In s vs) /\
+      (forall u v,
+          graph.edge g u v ->
+          In u vs' ->
+          ~ In u vs ->
+          graph.edge g_acc u v) /\
+      (forall u v, graph.edge g_acc u v -> graph.edge g u v).
 
 
-      Definition state' : Type := list V * state.
-      Definition untree_edge_upd' '(vs, st) v := (vs, untree_edge_upd st vs v).
-      Definition tree_edge_upd' '(vs, st) v := (v :: vs, tree_edge_upd st vs v).
-      Definition finish' '(vs, st) v := (vs, finish st vs v).
+  Lemma graph_corresp_eq vs g g_acc :
+    graph_corresp [] vs g g_acc ->
+    (forall u v, graph.edge g_acc u v <-> graph.edge g u v /\ In u vs).
+  Proof.
+    cbv [graph_corresp]. intros. fwd. split.
+    - intros. especialize Hp0.
+      { apply graph.sources_spec. eauto. }
+      fwd. auto.
+    - intros. fwd. auto.
+  Qed.
 
-      Definition already_seen (st' : state') v :=
-        let '(vs, _) := st' in set_contains vs v.
+  Definition weak_graph_corresp root root_edges vs vs' (g g_acc : graph) :=
+    (forall s, In s (graph.sources g_acc) -> In s vs'/\  ~In s vs) /\
+      (forall u v,
+          graph.edge g u v ->
+          In u vs' ->
+          ~ In u vs ->
+          u <> root ->
+          graph.edge g_acc u v) /\
+      (forall v, graph.edge g_acc root v <-> In v root_edges) /\
+      (forall u v, graph.edge g_acc u v -> graph.edge g u v).
 
-      Fixpoint dfs_fold' n st' v : state' :=
-        match n with
-        | S n' =>
-            if already_seen st' v then untree_edge_upd' st' v else
-              finish' (fold_left (dfs_fold' n') (graph.edges g v) (tree_edge_upd' st' v)) v
-        | O => st'
-        end.
+  Definition no_long_paths (g : graph) root vs n :=
+    forall p,
+      graph.path g root p ->
+      NoDup (root :: p) ->
+      Forall (fun v => ~In v vs) (root :: p) ->
+      S (S (length p)) < n.
 
-      Definition dfs_fold st0 := dfs_fold' (3 + length (graph.sources g)) ([], st0).
-    End with_graph.
+  Lemma no_long_paths_step g u v vs n :
+    no_long_paths g u vs (S n) ->
+    ~In u vs ->
+    graph.edge g u v ->
+    no_long_paths g v (u :: vs) n.
+  Proof.
+    cbv [no_long_paths]. intros H Hu He p Hp1 Hp2 Hp3.
+    specialize (H (v :: p)). simpl in H. especialize H.
+    - auto.
+    - constructor; auto. intros H. rewrite Forall_forall in Hp3.
+      eapply Hp3; simpl; eauto.
+    - constructor; auto. eapply Forall_impl; [|eassumption].
+      simpl. auto.
+    - lia.
+  Qed.
 
-    Inductive dfs_fold_state (root : V) vs0 st0 : list V (*seen*) -> state -> list V (*current path*)-> graph (*explored edges*) -> Prop :=
-    | dfs_init : dfs_fold_state _ _ _ vs0 st0 [root] graph.empty
-    | dfs_tree_edge vs st u p g v :
-      ~graph.edge g u v ->
-      dfs_fold_state _ _ _ vs st (u :: p) g ->
-      set_contains vs v = false ->
-      dfs_fold_state _ _ _ (v :: vs) (tree_edge_upd st vs v) (v :: u :: p) (graph.put g u v)
-    | dfs_untree_edge vs st u p g v :
-      dfs_fold_state _ _ _ vs st (u :: p) g ->
-      ~graph.edge g u v ->
-      set_contains vs v = true ->
-      dfs_fold_state _ _ _ vs (untree_edge_upd st vs v) (u :: p) (graph.put g u v)
-    | dfs_finish vs st u p g :
-      dfs_fold_state _ _ _ vs st (u :: p) g ->
-      dfs_fold_state _ _ _ vs (finish st vs u) p g.
-
-    Lemma set_contains_cons_true v vs y :
-      set_contains vs y = true -> set_contains (v :: vs) y = true.
-    Proof. rewrite !set_contains_true. simpl. auto. Qed.
-
-    Lemma set_contains_head v vs :
-      set_contains (v :: vs) v = true.
-    Proof. apply set_contains_true. left. reflexivity. Qed.
-
-    Lemma seen_mono root vs0 st0 vs st p g y :
-      dfs_fold_state root vs0 st0 vs st p g ->
-      set_contains vs0 y = true ->
-      set_contains vs y = true.
-    Proof. intros H Hy. induction H; auto using set_contains_cons_true. Qed.
-
-    Lemma seen_mono' root vs0 st0 vs st p g :
-      dfs_fold_state root vs0 st0 vs st p g ->
-      incl vs0 vs.
-    Proof.
-      intros H x Hx. apply set_contains_true. eapply seen_mono; try eassumption.
-      apply set_contains_true. exact Hx.
-    Qed.
-
-    Hint Unfold graph.edge : core.
-    Lemma dfs_target_seen root vs0 st0 vs st p g x y :
-      dfs_fold_state root vs0 st0 vs st p g -> graph.edge g x y -> set_contains vs y = true.
-    Proof.
-      intro H. revert x y.
-      induction H; intros x y He.
-      - apply graph.edge_empty in He. contradiction.
-      - apply graph.edge_put in He. destruct He as [Hold | [_ Hvy]].
-        + apply set_contains_cons_true. eauto.
-        + subst y. apply set_contains_head.
-      - apply graph.edge_put in He. destruct He as [Hold | [_ Hvy]].
-        + eauto.
-        + subst y. assumption.
-      - eauto.
-    Qed.
-
-    Lemma dfs_path_seen root vs0 st0 vs st p g z :
-      set_contains vs0 root = true ->
-      dfs_fold_state root vs0 st0 vs st p g ->
-      In z p ->
-      set_contains vs z = true.
-    Proof.
-      intros Hroot H. revert z.
-      induction H; intros z Hz.
-      - destruct Hz as [<- | []]. exact Hroot.
-      - destruct Hz as [<- | Hz].
-        + apply set_contains_head.
-        + apply set_contains_cons_true. eauto.
-      - eauto.
-      - eauto using in_cons.
-    Qed.
-
-    Lemma dfs_path_unseen root vs0 st0 vs st p g z :
-      dfs_fold_state root vs0 st0 vs st p g -> In z p -> z = root \/ set_contains vs0 z = false.
-    Proof.
-      intro H. revert z.
-      induction H; intros z Hz.
-      - destruct Hz as [<- | []]. left. reflexivity.
-      - destruct Hz as [<- | Hz].
-        + right. apply set_contains_false. intro Hin.
-          match goal with He : dfs_fold_state _ _ _ _ _ _ _ |- _ =>
-            apply (seen_mono' _ _ _ _ _ _ _ He) in Hin end.
-          apply set_contains_true in Hin. congruence.
-        + eauto.
-      - eauto.
-      - eauto using in_cons.
-    Qed.
-
-    Lemma dfs_source_seen root vs0 st0 vs st p g x y :
-      set_contains vs0 root = true ->
-      dfs_fold_state root vs0 st0 vs st p g -> graph.edge g x y -> set_contains vs x = true.
-    Proof.
-      intros Hroot H. revert x y.
-      induction H; intros x y He.
-      - apply graph.edge_empty in He. destruct He.
-      - apply graph.edge_put in He. destruct He as [Hold | [Hxhd _]].
-        + apply set_contains_cons_true. eauto.
-        + subst x. apply set_contains_cons_true.
-          eapply dfs_path_seen; [ exact Hroot | eassumption | apply in_eq ].
-      - apply graph.edge_put in He. destruct He as [Hold | [Hxhd _]].
-        + eauto.
-        + subst x. eapply dfs_path_seen; [ exact Hroot | eassumption | apply in_eq ].
-      - eauto.
-    Qed.
-
-    Lemma dfs_fold_state_trans root vs0 st0 vs st vs' st' p p' g g' u :
-      dfs_fold_state root vs0 st0 vs st (u :: p) g ->
-      set_contains vs0 root = true ->
-      graph.edges g u = [] ->
-      dfs_fold_state u vs st vs' st' p' g' ->
-      dfs_fold_state root vs0 st0 vs' st' (p' ++ p) (graph.union g g').
-    Proof.
-      intros H1 Hroot Hedges H2.
-      induction H2.
-      - cbn [app]. rewrite graph.union_empty_r. exact H1.
-      - cbn [app]. rewrite graph.union_put_r. apply dfs_tree_edge.
-        + intro Hedge. apply graph.edge_union in Hedge. destruct Hedge as [Hg | Hg0].
-          * pose proof (dfs_target_seen _ _ _ _ _ _ _ _ _ H1 Hg) as Hs.
-            match goal with He : dfs_fold_state u _ _ _ _ _ _ |- _ =>
-              pose proof (seen_mono _ _ _ _ _ _ _ _ He Hs) end.
-            congruence.
-          * contradiction.
-        + eassumption.
-        + eassumption.
-      - cbn [app]. rewrite graph.union_put_r. apply dfs_untree_edge.
-        + eassumption.
-        + intro Hedge. apply graph.edge_union in Hedge. destruct Hedge as [Hg | Hg0].
-          * match goal with He : dfs_fold_state u _ _ _ _ _ _ |- _ =>
-              pose proof (dfs_path_unseen _ _ _ _ _ _ _ _ He (in_eq _ _)) as Hun end.
-            destruct Hun as [-> | Hun].
-            -- cbv [graph.edge] in Hg. rewrite Hedges in Hg. destruct Hg.
-            -- pose proof (dfs_source_seen _ _ _ _ _ _ _ _ _ Hroot H1 Hg) as Hsn. congruence.
-          * contradiction.
-        + eassumption.
-      - eapply dfs_finish. eassumption.
-    Qed.
-
-    Definition graph_corresp vs vs' (g g_acc : graph) :=
-      (forall s, In s (graph.sources g_acc) -> In s vs'/\  ~In s vs) /\
-        (forall u v,
-            graph.edge g u v ->
-            In u vs' ->
-            ~ In u vs ->
-            graph.edge g_acc u v) /\
-        (forall u v, graph.edge g_acc u v -> graph.edge g u v).
-
-
-    Lemma graph_corresp_eq vs g g_acc :
-      graph_corresp [] vs g g_acc ->
-      (forall u v, graph.edge g_acc u v <-> graph.edge g u v /\ In u vs).
-    Proof.
-      cbv [graph_corresp]. intros. fwd. split.
-      - intros. especialize Hp0.
-        { apply graph.sources_spec. eauto. }
-        fwd. auto.
-      - intros. fwd. auto.
-    Qed.
-
-    Definition weak_graph_corresp root root_edges vs vs' (g g_acc : graph) :=
-      (forall s, In s (graph.sources g_acc) -> In s vs'/\  ~In s vs) /\
-        (forall u v,
-            graph.edge g u v ->
-            In u vs' ->
-            ~ In u vs ->
-            u <> root ->
-            graph.edge g_acc u v) /\
-        (forall v, graph.edge g_acc root v <-> In v root_edges) /\
-        (forall u v, graph.edge g_acc u v -> graph.edge g u v).
-
-    Definition no_long_paths (g : graph) root vs n :=
-      forall p,
-        graph.path g root p ->
-        NoDup (root :: p) ->
-        Forall (fun v => ~In v vs) (root :: p) ->
-        S (S (length p)) < n.
-
-    Lemma no_long_paths_step g u v vs n :
-      no_long_paths g u vs (S n) ->
-      ~In u vs ->
-      graph.edge g u v ->
-      no_long_paths g v (u :: vs) n.
-    Proof.
-      cbv [no_long_paths]. intros H Hu He p Hp1 Hp2 Hp3.
-      specialize (H (v :: p)). simpl in H. especialize H.
-      - auto.
-      - constructor; auto. intros H. rewrite Forall_forall in Hp3.
-        eapply Hp3; simpl; eauto.
-      - constructor; auto. eapply Forall_impl; [|eassumption].
-        simpl. auto.
-      - lia.
-    Qed.
-
-    Lemma no_long_paths_incl g u vs vs' n :
-      no_long_paths g u vs n ->
-      incl vs vs' ->
-      no_long_paths g u vs' n.
-    Proof.
-      cbv [no_long_paths]. intros. apply H; auto.
-      eapply Forall_impl; simpl; eauto. simpl. unfold not. auto.
-    Qed.
+  Lemma no_long_paths_incl g u vs vs' n :
+    no_long_paths g u vs n ->
+    incl vs vs' ->
+    no_long_paths g u vs' n.
+  Proof.
+    cbv [no_long_paths]. intros. apply H; auto.
+    eapply Forall_impl; simpl; eauto. simpl. unfold not. auto.
+  Qed.
 
 
 
-    Lemma no_long_paths_nonzero g root vs n :
-      no_long_paths g root vs n ->
-      ~In root vs ->
-      1 < n.
-    Proof.
-      cbv [no_long_paths]. intros H. specialize (H []). intro. subst.
-      especialize H; simpl; auto.
-      - constructor; auto. constructor.
-      - lia.
-    Qed.
+  Lemma no_long_paths_nonzero g root vs n :
+    no_long_paths g root vs n ->
+    ~In root vs ->
+    1 < n.
+  Proof.
+    cbv [no_long_paths]. intros H. specialize (H []). intro. subst.
+    especialize H; simpl; auto.
+    - constructor; auto. constructor.
+    - lia.
+  Qed.
 
-    Lemma dfs_fold'_sound root vs n st0 g vs' st' :
-      no_long_paths g root vs n ->
-      set_contains vs root = false ->
-      dfs_fold' g n (vs, st0) root = (vs', st') ->
-      exists g_acc,
-        dfs_fold_state root (root :: vs) (tree_edge_upd st0 vs root) vs' st' [] g_acc /\
-          graph_corresp vs vs' g g_acc.
-    Proof.
-      revert root vs st0 vs' st'. induction n.
-      { intros *. intros Hn Hroot. exfalso. cbv [no_long_paths] in Hn.
-        specialize (Hn []). simpl in Hn. especialize Hn; auto.
-        - constructor; simpl; auto. constructor.
-        - apply set_contains_false in Hroot. auto.
-        - lia. }
-      intros root vs st0 vs' st' Hn Hroot H.
-      assert (n <> 0).
-      { eapply no_long_paths_nonzero in Hn. 1: lia.
-        apply set_contains_false. assumption. }
-      simpl in H. simpl. rewrite Hroot in *.
-      cbv [finish'] in H. Tactics.destruct_one_match_hyp. fwd.
-      eenough (exists g_acc, _ /\ weak_graph_corresp root (rev (graph.edges g root)) vs vs' g g_acc) as [g_acc H].
-      { exists g_acc. split.
-        - apply dfs_finish. eapply (proj1 H).
-        - destruct H as [_ H].
-          cbv [graph_corresp].
-          cbv [weak_graph_corresp] in H. fwd. split; auto. split; auto. intros.
-          destruct (eqb_boolspec _ u root) as [Hu | Hu].
-          { subst. apply Hp2. rewrite <- in_rev. assumption. }
-          apply Hp1; assumption. }
-      rewrite <- fold_left_rev_right in E.
-      revert vs' s E.
-      apply fold_right_inv_NoDup.
-      - apply NoDup_rev. apply graph.edges_NoDup.
-      - intros. fwd. eexists. split; [constructor|].
-        cbv [weak_graph_corresp]. split.
-        { rewrite graph.sources_empty. simpl. contradiction. }
-        split; cycle 1.
-        { setoid_rewrite graph.edge_empty_iff. graph. }
-        intros. exfalso. destruct H1; subst; auto.
-      - intros * Hnotin Hin H * Hdfs. destruct a'.
-        specialize (H _ _ eq_refl). fwd. apply in_rev in Hin.
-        destruct (set_contains l b) eqn:Eb.
-        { destruct n; [lia|]. simpl in Hdfs. rewrite Eb in Hdfs. fwd.
-          eexists. split.
-          - apply dfs_untree_edge.
-            + eassumption.
-            + intro. apply Hnotin. cbv [weak_graph_corresp] in Hp1. fwd.
-              apply Hp1p2. assumption.
-            + simpl. assumption.
-          - cbv [weak_graph_corresp] in *. fwd. ssplit.
-            + cbv [incl]. intros v Hv. apply graph.sources_put in Hv. destruct Hv; auto.
-              subst. eapply seen_mono in Hp0.
-              -- apply set_contains_true in Hp0. split; [exact Hp0|].
-                 apply set_contains_false in Hroot. assumption.
-              -- apply set_contains_head.
-            + intros. rewrite graph.edge_put. left.
-              apply Hp1p1; auto.
-            + intros. rewrite graph.edge_put, Hp1p2.
-              simpl. split; intros [?|?]; fwd; auto.
-            + intros * H. apply graph.edge_put in H.
-              destruct H as [H|H]; fwd; auto. }
-        apply IHn in Hdfs.
-        + fwd.
-          eexists. split.
-          -- eapply dfs_fold_state_trans with (p' := nil).
-             ++ apply dfs_tree_edge. 2: eassumption.
-                --- intros H. cbv [weak_graph_corresp] in Hp1. fwd. apply Hp1p2 in H.
-                    eauto.
-                --- simpl. assumption.
-             ++ simpl. rewrite eqb_refl_true by assumption. reflexivity.
-             ++ apply forall_not_in_nil. intros v Hv. apply graph.edge_put in Hv.
-                destruct Hv as [H|H].
-                --- cbv [weak_graph_corresp] in Hp1. fwd.
-                    apply graph.edge_in_sources, Hp1p0 in H.
-                    apply set_contains_false in Eb. fwd. auto.
-                --- fwd. eapply seen_mono in Hp0; cycle 1.
-                    { apply set_contains_head. }
-                    congruence.
-             ++ eassumption.
-          -- cbv [weak_graph_corresp]. cbv [weak_graph_corresp] in Hp1. fwd.
-             apply seen_mono' in Hp0, Hdfsp0.
-             ssplit.
-             ++ cbv [incl]. intros v Hv. rewrite graph.sources_union, graph.sources_put in Hv.
-                destruct Hv as [[Hv|Hv]|Hv].
-                --- apply Hp1p0 in Hv. fwd. split; auto. apply Hdfsp0. simpl. auto.
-                --- subst. split.
-                    +++ apply Hdfsp0. simpl. right. apply Hp0. simpl. auto.
-                    +++ apply set_contains_false in Hroot. exact Hroot.
-                --- cbv [graph_corresp] in Hdfsp1. fwd. apply Hdfsp1p0 in Hv. fwd.
-                    split; auto. intro. apply Hvp1. apply Hp0. simpl. auto.
-             ++ intros. rewrite graph.edge_union, graph.edge_put.
-                destruct (set_contains l u) eqn:Hu;
-                  [apply set_contains_true in Hu | apply set_contains_false in Hu].
-                --- left. left. apply Hp1p1; auto.
-                --- right. apply Hdfsp1; auto.
-             ++ intros. rewrite graph.edge_union, graph.edge_put.
-                split.
-                --- intros [[Hv|Hv]|Hv].
-                    +++ simpl. right. apply Hp1p2. assumption.
-                    +++ fwd. simpl. auto.
-                    +++ cbv [graph_corresp] in Hdfsp1. fwd.
-                        apply graph.edge_in_sources, Hdfsp1p0 in Hv. fwd.
-                        exfalso. apply Hvp1. apply Hp0. simpl. auto.
-                --- intros [Hv|Hv].
-                    +++ subst. auto.
-                    +++ left. left. apply Hp1p2. assumption.
-             ++ intros. rewrite graph.edge_union, graph.edge_put in H.
-                destruct H as [[H|H]|H]; fwd; auto.
-                cbv [graph_corresp] in Hdfsp1. fwd. auto.
-        + eapply no_long_paths_incl.
-          -- apply no_long_paths_step; try eassumption.
-             apply set_contains_false in Hroot. exact Hroot.
-          -- apply seen_mono' in Hp0. exact Hp0.
-        + assumption.
-    Qed.
+  Lemma dfs_fold'_sound root vs n st0 g vs' st' :
+    no_long_paths g root vs n ->
+    set_contains vs root = false ->
+    dfs_fold' g n (vs, st0) root = (vs', st') ->
+    exists g_acc,
+      dfs_fold_state root (root :: vs) (tree_edge_upd st0 vs root) vs' st' [] g_acc /\
+        graph_corresp vs vs' g g_acc.
+  Proof.
+    revert root vs st0 vs' st'. induction n.
+    { intros *. intros Hn Hroot. exfalso. cbv [no_long_paths] in Hn.
+      specialize (Hn []). simpl in Hn. especialize Hn; auto.
+      - constructor; simpl; auto. constructor.
+      - apply set_contains_false in Hroot. auto.
+      - lia. }
+    intros root vs st0 vs' st' Hn Hroot H.
+    assert (n <> 0).
+    { eapply no_long_paths_nonzero in Hn. 1: lia.
+      apply set_contains_false. assumption. }
+    simpl in H. simpl. rewrite Hroot in *.
+    cbv [finish'] in H. Tactics.destruct_one_match_hyp. fwd.
+    eenough (exists g_acc, _ /\ weak_graph_corresp root (rev (graph.edges g root)) vs vs' g g_acc) as [g_acc H].
+    { exists g_acc. split.
+      - apply dfs_finish. eapply (proj1 H).
+      - destruct H as [_ H].
+        cbv [graph_corresp].
+        cbv [weak_graph_corresp] in H. fwd. split; auto. split; auto. intros.
+        destruct (eqb_boolspec _ u root) as [Hu | Hu].
+        { subst. apply Hp2. rewrite <- in_rev. assumption. }
+        apply Hp1; assumption. }
+    rewrite <- fold_left_rev_right in E.
+    revert vs' s E.
+    apply fold_right_inv_NoDup.
+    - apply NoDup_rev. apply graph.edges_NoDup.
+    - intros. fwd. eexists. split; [constructor|].
+      cbv [weak_graph_corresp]. split.
+      { rewrite graph.sources_empty. simpl. contradiction. }
+      split; cycle 1.
+      { setoid_rewrite graph.edge_empty_iff. graph. }
+      intros. exfalso. destruct H1; subst; auto.
+    - intros * Hnotin Hin H * Hdfs. destruct a'.
+      specialize (H _ _ eq_refl). fwd. apply in_rev in Hin.
+      destruct (set_contains l b) eqn:Eb.
+      { destruct n; [lia|]. simpl in Hdfs. rewrite Eb in Hdfs. fwd.
+        eexists. split.
+        - apply dfs_untree_edge.
+          + eassumption.
+          + intro. apply Hnotin. cbv [weak_graph_corresp] in Hp1. fwd.
+            apply Hp1p2. assumption.
+          + simpl. assumption.
+        - cbv [weak_graph_corresp] in *. fwd. ssplit.
+          + cbv [incl]. intros v Hv. apply graph.sources_put in Hv. destruct Hv; auto.
+            subst. eapply seen_mono in Hp0.
+            -- apply set_contains_true in Hp0. split; [exact Hp0|].
+               apply set_contains_false in Hroot. assumption.
+            -- apply set_contains_head.
+          + intros. rewrite graph.edge_put. left.
+            apply Hp1p1; auto.
+          + intros. rewrite graph.edge_put, Hp1p2.
+            simpl. split; intros [?|?]; fwd; auto.
+          + intros * H. apply graph.edge_put in H.
+            destruct H as [H|H]; fwd; auto. }
+      apply IHn in Hdfs.
+      + fwd.
+        eexists. split.
+        -- eapply dfs_fold_state_trans with (p' := nil).
+           ++ apply dfs_tree_edge. 2: eassumption.
+              --- intros H. cbv [weak_graph_corresp] in Hp1. fwd. apply Hp1p2 in H.
+                  eauto.
+              --- simpl. assumption.
+           ++ simpl. rewrite eqb_refl_true by assumption. reflexivity.
+           ++ apply forall_not_in_nil. intros v Hv. apply graph.edge_put in Hv.
+              destruct Hv as [H|H].
+              --- cbv [weak_graph_corresp] in Hp1. fwd.
+                  apply graph.edge_in_sources, Hp1p0 in H.
+                  apply set_contains_false in Eb. fwd. auto.
+              --- fwd. eapply seen_mono in Hp0; cycle 1.
+                  { apply set_contains_head. }
+                  congruence.
+           ++ eassumption.
+        -- cbv [weak_graph_corresp]. cbv [weak_graph_corresp] in Hp1. fwd.
+           apply seen_mono' in Hp0, Hdfsp0.
+           ssplit.
+           ++ cbv [incl]. intros v Hv. rewrite graph.sources_union, graph.sources_put in Hv.
+              destruct Hv as [[Hv|Hv]|Hv].
+              --- apply Hp1p0 in Hv. fwd. split; auto. apply Hdfsp0. simpl. auto.
+              --- subst. split.
+                  +++ apply Hdfsp0. simpl. right. apply Hp0. simpl. auto.
+                  +++ apply set_contains_false in Hroot. exact Hroot.
+              --- cbv [graph_corresp] in Hdfsp1. fwd. apply Hdfsp1p0 in Hv. fwd.
+                  split; auto. intro. apply Hvp1. apply Hp0. simpl. auto.
+           ++ intros. rewrite graph.edge_union, graph.edge_put.
+              destruct (set_contains l u) eqn:Hu;
+                [apply set_contains_true in Hu | apply set_contains_false in Hu].
+              --- left. left. apply Hp1p1; auto.
+              --- right. apply Hdfsp1; auto.
+           ++ intros. rewrite graph.edge_union, graph.edge_put.
+              split.
+              --- intros [[Hv|Hv]|Hv].
+                  +++ simpl. right. apply Hp1p2. assumption.
+                  +++ fwd. simpl. auto.
+                  +++ cbv [graph_corresp] in Hdfsp1. fwd.
+                      apply graph.edge_in_sources, Hdfsp1p0 in Hv. fwd.
+                      exfalso. apply Hvp1. apply Hp0. simpl. auto.
+              --- intros [Hv|Hv].
+                  +++ subst. auto.
+                  +++ left. left. apply Hp1p2. assumption.
+           ++ intros. rewrite graph.edge_union, graph.edge_put in H.
+              destruct H as [[H|H]|H]; fwd; auto.
+              cbv [graph_corresp] in Hdfsp1. fwd. auto.
+      + eapply no_long_paths_incl.
+        -- apply no_long_paths_step; try eassumption.
+           apply set_contains_false in Hroot. exact Hroot.
+        -- apply seen_mono' in Hp0. exact Hp0.
+      + assumption.
+  Qed.
 
 
-    Lemma paths_limited g root :
-      no_long_paths g root [] (S (S (S (length (graph.sources g))))).
-    Proof.
-      cbv [no_long_paths]. intros p H1 H2 _. apply graph.path_in_graph in H1.
-      apply NoDup_removelast in H2. eapply NoDup_incl_length in H2; [|eassumption].
-      rewrite length_removelast_cons in H2. lia.
-    Qed.
+  Lemma paths_limited g root :
+    no_long_paths g root [] (S (S (S (length (graph.sources g))))).
+  Proof.
+    cbv [no_long_paths]. intros p H1 H2 _. apply graph.path_in_graph in H1.
+    apply NoDup_removelast in H2. eapply NoDup_incl_length in H2; [|eassumption].
+    rewrite length_removelast_cons in H2. lia.
+  Qed.
 
-    Lemma dfs_fold_sound g st0 root vs st :
-      dfs_fold g st0 root = (vs, st) ->
-      exists g_acc,
-        dfs_fold_state root (root :: []) (tree_edge_upd st0 [] root) vs st [] g_acc /\
-          (forall u v, graph.edge g_acc u v <-> graph.edge g u v /\ In u vs).
-    Proof.
-      intros H. apply dfs_fold'_sound in H; cycle 1.
-      { apply paths_limited. }
-      { reflexivity. }
-      fwd. eauto using graph_corresp_eq.
-    Qed.
+  Lemma dfs_fold_sound g st0 root vs st :
+    dfs_fold g st0 root = (vs, st) ->
+    exists g_acc,
+      dfs_fold_state root (root :: []) (tree_edge_upd st0 [] root) vs st [] g_acc /\
+        (forall u v, graph.edge g_acc u v <-> graph.edge g u v /\ In u vs).
+  Proof.
+    intros H. apply dfs_fold'_sound in H; cycle 1.
+    { apply paths_limited. }
+    { reflexivity. }
+    fwd. eauto using graph_corresp_eq.
+  Qed.
 
   Lemma dfs_fold'_mono g n vs st root vs' st' :
     dfs_fold' g n (vs, st) root = (vs', st') ->
@@ -493,10 +488,9 @@ Section __.
     destruct H1 as [[]|?]. assumption.
   Qed.
 
-  Lemma dfs_fold_explores_everything g st root vs u v st' :
+  Lemma dfs_fold_explores_everything g st root vs u st' :
     dfs_fold g st root = (vs, st') ->
     graph.reaches g root u ->
-    graph.edge g u v ->
     In u vs.
   Proof.
     intros. cbv [dfs_fold plus] in H. eapply graph.edge_closed_reaches_in; cycle 1.
@@ -507,7 +501,7 @@ Section __.
     apply paths_limited.
   Qed.
 
-  Definition dfs_fold_spec g st0 root vs st :
+  Lemma dfs_fold_spec g st0 root vs st :
     dfs_fold g st0 root = (vs, st) ->
     exists g',
       graph.reachable_subgraph g root g' /\
@@ -616,5 +610,4 @@ Section __.
   Proof.
     eauto 8 using dfs_fold_state_p_good, dfs_fold_state_root_seen, dfs_fold_state_vs_good, dfs_fold_state_all_reachable.
   Qed.
-  End fold.
 End __.
